finished implementing maxnode

Examples/Kruskal/Kruskal_Final.thy
@@ -1,28 +1,26 @@
 theory Kruskal_Final
-imports Union_Find_Time Kruskal_Impl "SepLogicTime_RBTreeBasic.MergeSort_Impl"
-begin
+  imports Union_Find_Time Kruskal_Impl "SepLogicTime_RBTreeBasic.MergeSort_Impl"
+  "../Remdups"
+begin  
 
 
 datatype wrap = W (extr: "(nat \<times> int \<times> nat)")
 
 instantiation wrap :: linorder
 begin
-fun less_eq_wrap  where "less_eq_wrap (W (a2,a,a3)) (W (b2,b,b3)) = lexordp (\<le>) [a,a2,a3] [b,b2,b3]"
-fun less_wrap  where "less_wrap (W (a2,a,a3)) (W (b2,b,b3)) = lexordp (<) [a,a2,a3] [b,b2,b3]"
+fun less_eq_wrap  where "less_eq_wrap (W (a2,a,a3)) (W (b2,b,b3)) = (if a=b then (if a2=b2 then (if a3=b3 then True else a3<b3) else a2<b2) else a<b)"
+fun less_wrap  where "less_wrap (W (a2,a,a3)) (W (b2,b,b3)) = (if a=b then (if a2=b2 then (if a3=b3 then False else a3<b3) else a2<b2) else a<b)"
 
 
 instance  
   apply standard
   subgoal for x y apply(cases x; cases y) 
-      subgoal for xa xaa apply(cases xa; cases xaa) apply auto 
+      subgoal for xa xaa apply(cases xa; cases xaa) by auto done
   subgoal for x   apply(cases x ) by auto 
-  subgoal for x y z apply(cases x; cases y; cases z) by auto 
-  subgoal for x y apply(cases x; cases y) apply auto 
-    subgoal for x y apply(cases x; cases y) by auto  
-
-    sorry
+  subgoal for x y z apply(cases x; cases y; cases z)  subgoal for xa xaa xb apply(cases xa; cases xaa; cases xb) by (auto split: if_splits) done
+  subgoal for x y apply(cases x; cases y) by (auto split: if_splits) 
+  subgoal for x y apply(cases x; cases y) by auto  
   done
-  sorry
 end
 
 
@@ -78,14 +76,35 @@ lemma maxn_rule: "<p\<mapsto>\<^sub>axs * timeCredit_assn(length xs*2+2)> maxn p
   unfolding maxn_def by(sep_auto heap: maxn'_rule length_rule simp: zero_time) 
 
 
+thm destroy_rule remdups_rule
+
+term remdups_impl
+
+definition sortEdges'  :: "(nat \<times> int \<times> nat) list \<Rightarrow> ((nat \<times> int \<times> nat) list * nat) Heap"  where
+  "sortEdges' l = do {
+      da \<leftarrow> remdups_impl (map W l);
+      a \<leftarrow> destroy da;
+      merge_sort_impl a;
+      mn \<leftarrow> maxn a; 
+      sl \<leftarrow> Array.freeze a;
+      return (map extr sl, mn)
+    }"
+
+
+definition sortEdges'_time :: "nat \<Rightarrow> nat" where
+  "sortEdges'_time n = remdups_time n + 3 + merge_sort_time n + (n*2+2) +  (n+1) + 1"
+
+
 definition sortEdges  :: "(nat \<times> int \<times> nat) list \<Rightarrow> ((nat \<times> int \<times> nat) list * nat) Heap"  where
   "sortEdges l = do {
       a \<leftarrow> Array.of_list (map W l);
       merge_sort_impl a;
       mn \<leftarrow> maxn a; 
       sl \<leftarrow> Array.freeze a;
-      return (map extr sl, 0)
+      return (map extr sl, mn)
     }"
+
+
 
 definition sortEdges_time :: "nat \<Rightarrow> nat" where
   "sortEdges_time n = (n+1) + merge_sort_time n + (n*2+2) +  (n+1) + 1"
@@ -106,25 +125,168 @@ lemma maxn_sort_maprule: "<p\<mapsto>\<^sub>asort (map f xs) * timeCredit_assn(l
   using maxn_rule[where xs="sort (map f xs)"] by auto
 
 
+lemma sorted_wrap: "sorted_wrt Kruskal_Refine.edges_less_eq (map extr (sort l))"
+proof -
+  have "sorted (sort l)"   using sorted_sort by auto
+  with sorted_sorted_wrt have A: "sorted_wrt (\<le>) (sort l)" by metis 
+
+  have p: "\<And>x y. x \<le> y \<Longrightarrow>  Kruskal_Refine.edges_less_eq (extr x) (extr y) "
+    subgoal for x y
+      apply(cases x; cases y) apply (simp add: Kruskal_Refine.edges_less_eq_def)
+      subgoal for xa xaa apply(cases xa; cases xaa) by (auto split: if_splits)
+      done
+    done
+
+  show ?thesis
+    apply(simp add: sorted_wrt_map)
+    apply(rule sorted_wrt_mono_rel[OF _ A])
+    using  p by blast
+qed
+
+
+lemma extrW: "x \<in> S \<Longrightarrow> x \<in> extr ` W ` S "
+  unfolding extr_def  
+  by (metis extr_def imageI wrap.sel)  
+
+lemma extr_W_on_set: "extr ` W ` S = S"
+  by (auto simp: extrW)
+
 lemma freeze_sort_maprule:
   "<a \<mapsto>\<^sub>a sort (map f xs) * timeCredit_assn(1 + length xs)> Array.freeze a <\<lambda>r. a \<mapsto>\<^sub>a sort (map f xs) * \<up>(r = sort (map f xs))>" 
   using freeze_rule[where xs="sort (map f xs)"] by auto
 
 lemma sortEdges_rule: "<timeCredit_assn(sortEdges_time (length l))> sortEdges l <\<lambda>(sl, mn). \<up>(sorted_wrt edges_less_eq sl)>\<^sub>t"
   unfolding sortEdges_def  sortEdges_time_def
-  apply(sep_auto heap: mergeSort_map_rule maxn_sort_maprule of_list_map_rule  freeze_sort_maprule )
-  sorry
+  by(sep_auto heap: mergeSort_map_rule maxn_sort_maprule of_list_map_rule  freeze_sort_maprule simp: sorted_wrap )
+
+lemma sortEdges_rule2: "<timeCredit_assn(sortEdges_time (length l))> sortEdges l <\<lambda>(sl, mn). \<up>(set sl = set l \<and> mn=max_node l \<and> sorted_wrt edges_less_eq sl)>\<^sub>t"
+  unfolding sortEdges_def  sortEdges_time_def
+  apply(sep_auto heap: mergeSort_map_rule maxn_sort_maprule of_list_map_rule  freeze_sort_maprule simp: extrW sorted_wrap )
+  apply(simp add: max_node_def)
+  using extr_W_on_set    
+  by (metis (no_types, lifting) image_comp) 
+
+thm remdups_rule
+lemma remdup_map_rule:
+  "< timeCredit_assn (remdups_time (length l))> 
+          remdups_impl (map W l)
+        <\<lambda>r. \<exists>\<^sub>Ara. da_assn id_assn ra r * \<up> (set (map W l) = set ra \<and> distinct ra)>\<^sub>t"
+  using remdups_rule[where as="map W l"] by simp
+
+ 
+lemma da_assn_id: "da_assn id_assn = dyn_array" 
+  unfolding da_assn_def by simp   
 
 
+thm atake_time_def
 
-interpretation sortMaxnode sortEdges sort_time'
+lemma atake_time_mono: "x\<le>y \<Longrightarrow> atake_time x \<le> atake_time y" by(auto simp: atake_time_def)
+lemma adrop_time_mono: "x\<le>y \<Longrightarrow> adrop_time x \<le> adrop_time y" by(auto simp: adrop_time_def)
+lemma mergeinto_time_mono: "x\<le>y \<Longrightarrow> mergeinto_time x \<le> mergeinto_time y" by(auto simp: mergeinto_time_def)
+
+lemma merge_sort_time_mono: "x\<le>y \<Longrightarrow> merge_sort_time x \<le> merge_sort_time y"
+proof(induct y arbitrary: x rule: less_induct)
+  case (less y)
+  then show ?case
+  proof (cases "y\<le>1")
+    case   True
+    note t=this
+    with less show ?thesis by simp   
+  next
+    case f: False
+    then show ?thesis
+    proof(cases "x\<le>1")
+      case True
+      with f show ?thesis by (simp add: atake_time_def)
+    next
+      case False 
+      from False f less(2) show ?thesis apply (simp add:  )
+        by(auto intro!: add_mono intro: atake_time_mono adrop_time_mono mergeinto_time_mono less(1)) 
+    qed
+  qed
+qed 
+
+lemma mergeSort_smaller_rule:   
+  shows
+  "length ra \<le>  ll \<Longrightarrow>
+  <p \<mapsto>\<^sub>a ra * timeCredit_assn(merge_sort_time ll)>
+   merge_sort_impl p
+   <\<lambda>_. p \<mapsto>\<^sub>a sort ra>\<^sub>t"  
+  apply(rule ht_cons_rule[where P'="p \<mapsto>\<^sub>a ra * timeCredit_assn (merge_sort_time (length ra)) * true"])
+    apply(simp only: mult.assoc)
+    apply(rule match_first)  apply(rule gc_time)
+  apply(rule merge_sort_time_mono) apply simp
+  defer  apply(rule fi_rule[where F=true]) apply(rule mergeSort_correct[where xs="ra"])
+   apply sep_auto+
+  done
+
+lemma maxn_sort_smallerrule: "length xs \<le> S \<Longrightarrow> <p\<mapsto>\<^sub>axs * timeCredit_assn(S*2+2)> maxn p <\<lambda>r. p\<mapsto>\<^sub>axs *  \<up>(r=maxnode  (map extr xs))>\<^sub>t"
+  apply(rule ht_cons_rule[where P'="p \<mapsto>\<^sub>a xs * timeCredit_assn (2*(length xs)+2) * true"])
+    apply(simp only: mult.assoc)
+    apply(rule match_first)  apply(rule gc_time)  apply simp
+  defer  apply(rule fi_rule[where F=true]) apply(rule maxn_rule[where xs="xs"])
+   apply sep_auto+
+  done 
+
+lemma freeze_smallerrule: "length xs \<le> S \<Longrightarrow> <a \<mapsto>\<^sub>a xs * timeCredit_assn(1 + S)> Array.freeze a <\<lambda>r. a \<mapsto>\<^sub>a xs * \<up>(r = xs)>\<^sub>t"
+  apply(rule ht_cons_rule[where P'="a \<mapsto>\<^sub>a xs * timeCredit_assn (1+(length xs)) * true"])
+    apply(simp only: mult.assoc)
+    apply(rule match_first)  apply(rule gc_time)  apply simp
+  defer  apply(rule fi_rule[where F=true]) apply(rule freeze_rule[where xs="xs"])
+   apply sep_auto+
+  done 
+ 
+
+lemma distinct_sort: "distinct a \<Longrightarrow> distinct (sort a)"   
+  by simp  
+
+lemma sortEdges'_rule: "<timeCredit_assn(sortEdges'_time (length l))>
+           sortEdges' l 
+      <\<lambda>(sl, mn). \<up>(sorted_wrt edges_less_eq sl \<and> set l = set sl \<and> distinct sl \<and> max_node l = mn)>\<^sub>t"
+  unfolding sortEdges'_def  sortEdges'_time_def
+  apply(sep_auto heap: remdup_map_rule) 
+   apply(rule fi_rule[where F="timeCredit_assn(7 + (3 * length l + ( merge_sort_time (length l))))", OF  ht_cons_rule[OF _ _ remdup_map_rule]])
+     apply (rule ent_refl) apply (rule ent_refl)
+  subgoal by (simp add: norm_assertion_simps dollarD)
+  apply(simp add: da_assn_id)                               
+  apply(sep_auto heap: destroy_rule remdup_map_rule mergeSort_map_rule maxn_sort_maprule of_list_map_rule  freeze_sort_maprule simp: sorted_wrap )
+   apply(sep_auto heap: mergeSort_smaller_rule[where ll="length l"])
+  subgoal  
+    by (metis distinct_length_le length_map set_map)  
+  apply(sep_auto heap: maxn_sort_smallerrule[where S="length l"])
+  subgoal 
+    by (metis distinct_length_le length_map set_map)  
+  apply(sep_auto heap: freeze_smallerrule[where S="length l"])
+  subgoal 
+    by (metis distinct_length_le length_map set_map)  
+  apply (sep_auto simp: sorted_wrap )
+  subgoal 
+    using extrW by blast 
+  subgoal  
+    using extr_W_on_set by blast   
+  subgoal apply(simp add: distinct_map)  
+    by (simp add: inj_onI wrap.expand)  
+  subgoal unfolding max_node_def 
+    using extr_W_on_set    
+    by (metis (no_types, lifting) image_comp)   
+  done 
+
+
+lemma ll: "list_assn id_assn   = pure Id" 
+  by (simp add: list_assn_pure_conv)  
+
+interpretation sortMaxnode sortEdges' sortEdges'_time
   apply(unfold_locales)
   apply (auto simp add: hfref_def mop_sortEdges_def)
   subgoal for t c a
-    apply(rule extract_cost_otherway'[OF _ sortEdges_rule, where Cost_lb="sortEdges_time (length c)"])
-    apply sep_auto
-     apply sep_auto
-    sorry
+    apply(rule extract_cost_otherway'[OF _ sortEdges'_rule, where Cost_lb="sortEdges'_time (length c)"])
+      apply sep_auto
+    subgoal 
+      apply (auto simp: list_assn_pure_conv   )
+      apply(simp add: pure_def) apply sep_auto unfolding max_node_def by simp
+    subgoal 
+      apply (auto simp: list_assn_pure_conv   ) apply(simp only: ran_emb' pure_def) by auto 
+    done
   done
 
 
